examples/FiniteSetsExamples.v
@@ -162,12 +162,6 @@ Proof.
   finish sharpening computation.
 Defined.
 
-Require Import Ensembles.
-Require Import Coq.Strings.String Coq.Sets.Ensembles Coq.Sets.Finite_sets Coq.Lists.List Coq.Sorting.Permutation.
-Require Import ADT ADT.ComputationalADT ADTRefinement.Core ADTNotation ADTRefinement.GeneralRefinements Common.AdditionalEnsembleDefinitions Common.AdditionalEnsembleLemmas Computation.
-Require Export FiniteSetADTs.FiniteSetADT.
-Require Import Common.
-
 Definition filterLtUniqueImpl2 (FiniteSetImpl : FullySharpened FiniteSetSpec) (ls : list W) (x : W)
 : FullySharpenedComputation (filterLtUniqueSpec2 ls x).
 Proof.
@@ -175,10 +169,14 @@ Proof.
 
   sharpen computation with FiniteSet implementation := FiniteSetImpl.
 
-  exfalso; admit;finish sharpening computation.
-  Grab Existential Variables.
-  admit.
+  finish sharpening computation.
 Defined.
+
+Require Import Ensembles.
+Require Import Coq.Strings.String Coq.Sets.Ensembles Coq.Sets.Finite_sets Coq.Lists.List Coq.Sorting.Permutation.
+Require Import ADT ADT.ComputationalADT ADTRefinement.Core ADTNotation ADTRefinement.GeneralRefinements Common.AdditionalEnsembleDefinitions Common.AdditionalEnsembleLemmas Computation.
+Require Export FiniteSetADTs.FiniteSetADT.
+Require Import Common.
 
 Definition intersectionUniqueImpl (FiniteSetImpl : FullySharpened FiniteSetSpec) (ls1 ls2 : list W)
 : FullySharpenedComputation (intersectionUniqueSpec ls1 ls2).
@@ -210,10 +208,6 @@ Proof.
   begin sharpening computation.
 
   sharpen computation with FiniteSet implementation := FiniteSetImpl.
-
-  (** TODO: create a synonym for [snd (FiniteSetAndFunctionOfList
-      FiniteSetImpl ...)], and then prove that it respects pointwise
-      refinement. *)
 
   exfalso; admit;finish sharpening computation.
   Grab Existential Variables.
